Source/IntegrationTests/TestFiles/LitTests/LitTest/proof-obligation-desc/read-array-allocation-invalid-read.dfy
@@ -1,4 +1,4 @@
-// RUN: %exits-with 2 %verify --type-system-refresh --general-traits=datatype --general-newtypes --reads-clauses-on-methods "%s" > "%t"
+// RUN: %exits-with 4 %verify --type-system-refresh --general-traits=datatype --general-newtypes --reads-clauses-on-methods "%s" > "%t"
 // RUN: %diff "%s.expect" "%t"
 
 method ReadUnapplied(c: Cell)
@@ -6,15 +6,36 @@ method ReadUnapplied(c: Cell)
 {
   if
   case true =>
-    var arr := new int[10](_ reads c => c.data); // error: insufficient reads
+    var arr := new int[10](_ reads c => c.data); // error: insufficient reads 
+  case true =>
+    var init := (i: int) reads c => 300;
+    var arr := new int[10](init); // error: insufficient reads 
+  case true =>
+    var arr := new int[10](c.IndexToElement); // error: insufficient reads 
 }
 
+method ReadUnappliedInArrayDimensionSizeExpressions(c: Cell)
+  reads {}
+{
+  if
+  case true =>
+    var arr := new int[ReadAnObject(c)](_ => 100); // error: insufficient reads 
+  case true =>
+    var arr := new int[ReadAnObject(c)] [20, 30, 40]; // error: insufficient reads 
+  case true =>
+    var arr := new int[3] [20, ReadAnObject(c), 40]; // error: insufficient reads 
+}
+  
 class Cell {
-  var data: int
+  var data: nat
+
+  function IndexToElement(i: int): int {
+    300
+  }
 }
 
-function ReadAnObject(c: Cell): int
+function ReadAnObject(c: Cell): nat
   reads c
 {
-  c.data
+  c.data + 3 - c.data
 }
